revise validPageDb, add unmap SVC, and prove some things
 * require <= 1 ref to each datapage
 * refactor other parts of validPageDb, because I couldn't resist
 * remove bizarro validPageNr constraints from validMapping
 * spec SVC call to unmap a data page
 * struggle through re-proving mapping.i and most of svcapi.i (proving things about dataPageRefs is painful!)

realised that I needed to add another constraint to validPageDb, to ensure that every L2 is linked in an L1

verified/kom_common.s.dfy
@@ -26,8 +26,8 @@ const KOM_SVC_VERIFY_STEP0:int      := 2;
 const KOM_SVC_VERIFY_STEP1:int      := 3;
 const KOM_SVC_VERIFY_STEP2:int      := 4;
 const KOM_SVC_MAP_DATA:int          := 10;
-const KOM_SVC_INIT_L2PTABLE:int     := 11;
-const KOM_SVC_UNMAP:int             := 12;
+const KOM_SVC_UNMAP_DATA:int        := 11;
+const KOM_SVC_INIT_L2PTABLE:int     := 12;
 
 //-----------------------------------------------------------------------------
 // Errors
