verified/mapping.i.dfy
@@ -1,40 +1,239 @@
 include "mapping.s.dfy"
 
-lemma installL1PTEPreservesPageDbValidity(pageDbIn: PageDb, l1ptnr: PageNr,
-                                          l2page: PageNr, l1index: int)
+lemma lemma_installL1PTEInPageDb_dataPageRefs(d1:PageDb, d2:PageDb, asPg: PageNr, l1ptnr: PageNr, l2page: PageNr, l1index: int, n:PageNr)
+    requires validPageDb(d1) && wellFormedPageDb(d2)
+    requires isAddrspace(d1, asPg) && !stoppedAddrspace(d1[asPg])
+    requires l1ptnr == d1[asPg].entry.l1ptnr
+    requires d1[l1ptnr].PageDbEntryTyped? && d1[l1ptnr].entry.L1PTable?
+    requires 0 <= l1index < NR_L1PTES
+    requires d1[l1ptnr].entry.l1pt[l1index].Nothing?
+    requires validL1PTE(d1, l2page) && d1[l2page].addrspace == d1[l1ptnr].addrspace
+    requires forall e | e in d1[l2page].entry.l2pt :: e.NoMapping?
+    requires d2 == installL1PTEInPageDb(d1, l1ptnr, l2page, l1index)
+    requires n != l1ptnr && n != l2page && l2page != l1ptnr
+    requires d1[n].PageDbEntryTyped? && d1[n].entry.DataPage?
+    requires !hasStoppedAddrspace(d1, n)
+    ensures isAddrspace(d1, d1[n].addrspace)
+    ensures dataPageRefs(d1, d1[n].addrspace, n) == dataPageRefs(d2, d2[n].addrspace, n)
+{
+    reveal validPageDb();
+    assert validPageDbEntryTyped(d1, n);
+    assert d2[n] == d1[n];
+    if d1[n].addrspace == asPg {
+        calc {
+            dataPageRefs(d1, d1[n].addrspace, n);
+            { assert d1[l1ptnr].PageDbEntryTyped? && d1[l1ptnr].entry.L1PTable?; }
+            (set i1, i2 {:trigger d1[d1[l1ptnr].entry.l1pt[i1].v].entry.l2pt[i2]} |
+                0 <= i1 < NR_L1PTES && 0 <= i2 < NR_L2PTES
+                && var l1e := d1[l1ptnr].entry.l1pt[i1]; l1e.Just?
+                && d1[l1e.v].PageDbEntryTyped? && d1[l1e.v].entry.L2PTable?
+                && var l2e := d1[l1e.v].entry.l2pt[i2]; l2e.SecureMapping?
+                && l2e.page == n :: (i1, i2));
+            { assert forall n:PageNr | n != l1ptnr :: d1[n] == d2[n]; }
+            (set i1, i2 {:trigger d2[d1[l1ptnr].entry.l1pt[i1].v].entry.l2pt[i2]} |
+                0 <= i1 < NR_L1PTES && 0 <= i2 < NR_L2PTES
+                && var l1e := d1[l1ptnr].entry.l1pt[i1]; l1e.Just?
+                && d2[l1e.v].PageDbEntryTyped? && d2[l1e.v].entry.L2PTable?
+                && var l2e := d2[l1e.v].entry.l2pt[i2]; l2e.SecureMapping?
+                && l2e.page == n :: (i1, i2));
+            {
+                var l1pt := d1[l1ptnr].entry.l1pt;
+                assert d2[l1ptnr].entry.l1pt == l1pt[l1index := Just(l2page)];
+                assert l1pt[l1index].Nothing?;
+                assert forall i1 | 0 <= i1 < NR_L1PTES && d2[l1ptnr].entry.l1pt[i1].Just?
+                    :: d2[l1ptnr].entry.l1pt[i1].v == l2page || d2[l1ptnr].entry.l1pt[i1] == l1pt[i1];
+                assert forall i2 | 0 <= i2 < NR_L2PTES :: d2[l2page].entry.l2pt[i2].NoMapping?;
+            }
+            (set i1, i2 {:trigger d2[d1[l1ptnr].entry.l1pt[i1].v].entry.l2pt[i2]} |
+                && 0 <= i1 < NR_L1PTES && 0 <= i2 < NR_L2PTES
+                && var l1e := d2[l1ptnr].entry.l1pt[i1]; l1e.Just?
+                && d2[l1e.v].PageDbEntryTyped? && d2[l1e.v].entry.L2PTable?
+                && var l2e := d2[l1e.v].entry.l2pt[i2]; l2e.SecureMapping?
+                && l2e.page == n :: (i1, i2));
+            dataPageRefs(d2, d2[n].addrspace, n);
+        }
+    } else { // different AS
+        var a := d1[n].addrspace;
+        var l1 := d1[a].entry.l1ptnr;
+        calc {
+            dataPageRefs(d1, a, n);
+            (set i1, i2 {:trigger d1[d1[l1].entry.l1pt[i1].v].entry.l2pt[i2]} |
+                d1[l1].PageDbEntryTyped? && d1[l1].entry.L1PTable?
+                && 0 <= i1 < NR_L1PTES && 0 <= i2 < NR_L2PTES
+                && var l1e := d1[l1].entry.l1pt[i1]; l1e.Just?
+                && d1[l1e.v].PageDbEntryTyped? && d1[l1e.v].entry.L2PTable?
+                && var l2e := d1[l1e.v].entry.l2pt[i2]; l2e.SecureMapping?
+                && l2e.page == n :: (i1, i2));
+            { assert l1 != l1ptnr; assert d1[a] == d2[a] && d1[l1] == d2[l1]; }
+            (set i1, i2 {:trigger d1[d2[l1].entry.l1pt[i1].v].entry.l2pt[i2]} |
+                d1[l1].PageDbEntryTyped? && d1[l1].entry.L1PTable?
+                && 0 <= i1 < NR_L1PTES && 0 <= i2 < NR_L2PTES
+                && var l1e := d2[l1].entry.l1pt[i1]; l1e.Just?
+                && d1[l1e.v].PageDbEntryTyped? && d1[l1e.v].entry.L2PTable?
+                && var l2e := d1[l1e.v].entry.l2pt[i2]; l2e.SecureMapping?
+                && l2e.page == n :: (i1, i2));
+            dataPageRefs(d2, a, n);
+        }
+    }
+}
+
+lemma lemma_installL1PTEPreservesPageDbValidity(pageDbIn: PageDb, asPg: PageNr,
+                                        l1ptnr: PageNr, l2page: PageNr, l1index: int)
     requires validPageDb(pageDbIn)
+    requires isAddrspace(pageDbIn, asPg) && !stoppedAddrspace(pageDbIn[asPg])
+    requires l1ptnr == pageDbIn[asPg].entry.l1ptnr
     requires pageDbIn[l1ptnr].PageDbEntryTyped? && pageDbIn[l1ptnr].entry.L1PTable?
-    // l2page belongs to this addrspace
+    // l2pt belongs to this addrspace, and is empty
     requires validL1PTE(pageDbIn, l2page)
-        && pageDbIn[l2page].addrspace == pageDbIn[l1ptnr].addrspace
+            && pageDbIn[l2page].addrspace == pageDbIn[l1ptnr].addrspace
+    requires forall e | e in pageDbIn[l2page].entry.l2pt :: e.NoMapping?
     // no double mapping
+    requires 0 <= l1index < NR_L1PTES
     requires forall i :: 0 <= i < NR_L1PTES && i != l1index
         ==> pageDbIn[l1ptnr].entry.l1pt[i] != Just(l2page)
-    requires 0 <= l1index < NR_L1PTES
+    requires pageDbIn[l1ptnr].entry.l1pt[l1index].Nothing?
     ensures validPageDb(installL1PTEInPageDb(pageDbIn, l1ptnr, l2page, l1index))
 {
     reveal validPageDb();
 
-    assert validL1PTable(pageDbIn, l1ptnr);
+    assert validL1PTable(pageDbIn, asPg, pageDbIn[l1ptnr].entry.l1pt);
     var pageDbOut := installL1PTEInPageDb(pageDbIn, l1ptnr, l2page, l1index);
+    assert validL1PTable(pageDbOut, asPg, pageDbOut[l1ptnr].entry.l1pt);
 
-    assert validL1PTable(pageDbOut, l1ptnr);
-
-    forall ( n | validPageNr(n) && n != l1ptnr)
+    forall (n | validPageNr(n) && n != l1ptnr)
         ensures validPageDbEntry(pageDbOut, n)
     {
         assert pageDbOut[n] == pageDbIn[n];
         assert validPageDbEntry(pageDbIn, n);
         assert addrspaceRefs(pageDbOut, n) == addrspaceRefs(pageDbIn, n);
+        if pageDbIn[n].PageDbEntryTyped? && pageDbIn[n].entry.DataPage?
+            && !hasStoppedAddrspace(pageDbIn, n) {
+            lemma_installL1PTEInPageDb_dataPageRefs(pageDbIn, pageDbOut, asPg,
+                                                    l1ptnr, l2page, l1index, n);
+        }
     }
 }
 
-lemma lemma_updateL2PtePreservesPageDb(d:PageDb,a:PageNr,mapping:Mapping,l2e:L2PTE) 
+predicate validAndEmptyMapping(m:Mapping, d:PageDb, a:PageNr)
+{
+    reveal validPageDb();
+    validMapping(m, d, a) &&
+    var addrspace := d[a].entry;
+    var l1pt := d[addrspace.l1ptnr].entry.l1pt;
+    var l2pt := d[l1pt[m.l1index].v].entry.l2pt;
+    l2pt[m.l2index].NoMapping?
+}
+
+lemma lemma_updateL2Pte_dataPageRefs(d1:PageDb, d2:PageDb, a:PageNr, mapping:Mapping, l2e:L2PTE, n:PageNr)
+    requires validPageDb(d1) && wellFormedPageDb(d2)
+    requires validMapping(mapping, d1, a) && validL2PTE(d1, a, l2e)
+    requires l2e.SecureMapping? ==>
+        validAndEmptyMapping(mapping, d1, a) && dataPageRefs(d1, a, l2e.page) == {}
+    requires d2 == updateL2Pte(d1, a, mapping, l2e)
+    requires d1[n].PageDbEntryTyped? && d1[n].entry.DataPage? && d1[n].addrspace == a
+    ensures |dataPageRefs(d2, a, n)| <= 1
+{
+    reveal validPageDb();
+    assert validPageDbEntryTyped(d1, n);
+    assert d2[n] == d1[n];
+
+    var l1ptnr := d1[a].entry.l1ptnr;
+    var l1pt := d1[l1ptnr].entry.l1pt;
+    var l2ptnr := l1pt[mapping.l1index].v;
+    var l2pt := d1[l2ptnr].entry.l2pt;
+    assert l2e.SecureMapping? ==> l2pt[mapping.l2index].NoMapping?;
+    var l2pt' := d2[l2ptnr].entry.l2pt;
+    assert l2pt' == l2pt[mapping.l2index := l2e];
+
+    if l2e.SecureMapping? && n == l2e.page { // same page: +1 refs
+        calc {
+            dataPageRefs(d1, a, n) + {(mapping.l1index, mapping.l2index)};
+            { assert d1[l1ptnr].PageDbEntryTyped? && d1[l1ptnr].entry.L1PTable?; }
+            (set i1, i2 {:trigger d1[l1pt[i1].v].entry.l2pt[i2]} |
+                0 <= i1 < NR_L1PTES && 0 <= i2 < NR_L2PTES
+                && var l1e := l1pt[i1]; l1e.Just?
+                && d1[l1e.v].PageDbEntryTyped? && d1[l1e.v].entry.L2PTable?
+                && var l2e := d1[l1e.v].entry.l2pt[i2]; l2e.SecureMapping?
+                && l2e.page == n :: (i1, i2)) + {(mapping.l1index, mapping.l2index)};
+            {
+                assert forall n:PageNr | n != l2ptnr :: d1[n] == d2[n];
+                assert dataPageRefs(d1, a, n) == {};
+            }
+            (set i1, i2 {:trigger d2[l1pt[i1].v].entry.l2pt[i2]} |
+                0 <= i1 < NR_L1PTES && 0 <= i2 < NR_L2PTES
+                && var l1e := l1pt[i1]; l1e.Just?
+                && d2[l1e.v].PageDbEntryTyped? && d2[l1e.v].entry.L2PTable?
+                && var l2e := d2[l1e.v].entry.l2pt[i2]; l2e.SecureMapping?
+                && l2e.page == n :: (i1, i2)) + {(mapping.l1index, mapping.l2index)};
+            {
+                assert forall i | 0 <= i < NR_L2PTES && l2pt'[i].SecureMapping? ::
+                    if i == mapping.l2index then l2pt'[i] == l2e
+                    else l2pt'[i] == l2pt[i];
+            }
+            (set i1, i2 {:trigger d2[l1pt[i1].v].entry.l2pt[i2]}
+                        {:trigger d2[d2[l1ptnr].entry.l1pt[i1].v].entry.l2pt[i2]} |
+                0 <= i1 < NR_L1PTES && 0 <= i2 < NR_L2PTES
+                && var l1e := l1pt[i1]; l1e.Just?
+                && d2[l1e.v].PageDbEntryTyped? && d2[l1e.v].entry.L2PTable?
+                && var l2e := d2[l1e.v].entry.l2pt[i2]; l2e.SecureMapping?
+                && l2e.page == n :: (i1, i2));
+            dataPageRefs(d2, a, n);
+        }
+    } else if l2pt[mapping.l2index].SecureMapping? && l2pt[mapping.l2index].page == n {
+        // replacing mapping: -1 refs
+        calc {
+            dataPageRefs(d1, a, n);
+            { assert d1[l1ptnr].PageDbEntryTyped? && d1[l1ptnr].entry.L1PTable?; }
+            (set i1, i2 {:trigger d1[l1pt[i1].v].entry.l2pt[i2]} |
+                0 <= i1 < NR_L1PTES && 0 <= i2 < NR_L2PTES
+                && var l1e := l1pt[i1]; l1e.Just?
+                && d1[l1e.v].PageDbEntryTyped? && d1[l1e.v].entry.L2PTable?
+                && var l2e := d1[l1e.v].entry.l2pt[i2]; l2e.SecureMapping?
+                && l2e.page == n :: (i1, i2));
+            {
+                assert forall n:PageNr | n != l2ptnr :: d1[n] == d2[n];
+                assert forall i | 0 <= i < NR_L2PTES && l2pt'[i].SecureMapping? ::
+                    l2pt'[i] == l2pt[i] || l2pt'[i] == l2e;
+            }
+            (set i1, i2 {:trigger d2[l1pt[i1].v].entry.l2pt[i2]} |
+                0 <= i1 < NR_L1PTES && 0 <= i2 < NR_L2PTES
+                && var l1e := l1pt[i1]; l1e.Just?
+                && d2[l1e.v].PageDbEntryTyped? && d2[l1e.v].entry.L2PTable?
+                && var l2e := d2[l1e.v].entry.l2pt[i2]; l2e.SecureMapping?
+                && l2e.page == n :: (i1, i2)) + {(mapping.l1index, mapping.l2index)};
+            dataPageRefs(d2, a, n) + {(mapping.l1index, mapping.l2index)};
+        }
+    } else {
+        calc {
+            dataPageRefs(d1, a, n);
+            { assert d1[l1ptnr].PageDbEntryTyped? && d1[l1ptnr].entry.L1PTable?; }
+            (set i1, i2 {:trigger d1[l1pt[i1].v].entry.l2pt[i2]} |
+                0 <= i1 < NR_L1PTES && 0 <= i2 < NR_L2PTES
+                && var l1e := l1pt[i1]; l1e.Just?
+                && d1[l1e.v].PageDbEntryTyped? && d1[l1e.v].entry.L2PTable?
+                && var l2e := d1[l1e.v].entry.l2pt[i2]; l2e.SecureMapping?
+                && l2e.page == n :: (i1, i2));
+            {
+                assert forall n:PageNr | n != l2ptnr :: d1[n] == d2[n];
+                assert forall i | 0 <= i < NR_L2PTES && l2pt'[i].SecureMapping? ::
+                    l2pt'[i] == l2pt[i] || l2pt'[i] == l2e;
+            }
+            (set i1, i2 {:trigger d2[l1pt[i1].v].entry.l2pt[i2]} |
+                0 <= i1 < NR_L1PTES && 0 <= i2 < NR_L2PTES
+                && var l1e := l1pt[i1]; l1e.Just?
+                && d2[l1e.v].PageDbEntryTyped? && d2[l1e.v].entry.L2PTable?
+                && var l2e := d2[l1e.v].entry.l2pt[i2]; l2e.SecureMapping?
+                && l2e.page == n :: (i1, i2));
+            dataPageRefs(d2, a, n);
+        }
+    }
+}
+
+lemma lemma_updateL2PtePreservesPageDb(d:PageDb,a:PageNr,mapping:Mapping,l2e:L2PTE)
     requires validPageDb(d)
-    requires isAddrspace(d, a)
-    requires validMapping(mapping,d,a)
-    requires !d[a].entry.state.StoppedState?
-    requires validL2PTE(d,a,l2e)
+    requires validMapping(mapping, d, a) && validL2PTE(d, a, l2e)
+    requires l2e.SecureMapping? ==>
+        validAndEmptyMapping(mapping, d, a) && dataPageRefs(d, a, l2e.page) == {}
     ensures validPageDb(updateL2Pte(d,a,mapping,l2e))
 {
     reveal validPageDb();
@@ -98,13 +297,22 @@ lemma lemma_updateL2PtePreservesPageDb(d:PageDb,a:PageNr,mapping:Mapping,l2e:L2P
     forall ( p | validPageNr(p) && p != l1p && p != l1pte && p != a )
         ensures validPageDbEntry(d', p)
     {
-            assert d'[p] == d[p];
-            assert validPageDbEntry(d, p);
-            assert addrspaceRefs(d', p) == addrspaceRefs(d, p);
+        assert d'[p] == d[p];
+        assert validPageDbEntry(d, p);
+        assert addrspaceRefs(d', p) == addrspaceRefs(d, p);
+        if d[p].PageDbEntryTyped? && d[p].entry.DataPage?
+            && !hasStoppedAddrspace(d, p) {
+            assert |dataPageRefs(d, d[p].addrspace, p)| <= 1;
+            if d[p].addrspace == a {
+                lemma_updateL2Pte_dataPageRefs(d, d', a, mapping, l2e, p);
+            } else { // diff AS
+                assert dataPageRefs(d, d[p].addrspace, p)
+                    == dataPageRefs(d', d[p].addrspace, p);
+            }
+        }
     }
     
     assert wellFormedPageDb(d');
     assert pageDbEntriesValid(d');
     assert pageDbEntriesValidRefs(d');
-  
 }
