verified/svcapi.s.dfy
@@ -60,16 +60,45 @@ lemma lemma_allocateSparePage(d:PageDb, p:PageNr, e:PageDbEntryTyped)
     requires d[p].PageDbEntryTyped? && d[p].entry.SparePage?
     requires wellFormedPageDbEntryTyped(e)
     requires e.DataPage? || e == L2PTable(SeqRepeat(NR_L2PTES, NoMapping))
+    requires !hasStoppedAddrspace(d, p)
     ensures validPageDb(allocateSparePage(d, p, e))
 {
     reveal validPageDb();
     var dOut := allocateSparePage(d, p, e);
 
-    forall (n:PageNr)
-        ensures validPageDbEntry(dOut, n)
+    forall (n:PageNr | dOut[n].PageDbEntryTyped?)
+        ensures validPageDbEntryTyped(dOut, n)
     {
         assert addrspaceRefs(dOut, n) == addrspaceRefs(d, n);
-        assert validPageDbEntry(d, n) && validPageDbEntry(dOut, n);
+        assert validPageDbEntryTyped(d, n);
+        var a := dOut[n].addrspace;
+        if !d[a].entry.state.StoppedState? {
+            var l1ptnr := d[a].entry.l1ptnr;
+            var l1pt := d[l1ptnr].entry.l1pt;
+            if n == p {
+                if e.DataPage? {
+                    assert forall i, j | 0 <= i < NR_L1PTES && l1pt[i].Just?
+                                             && 0 <= j < NR_L2PTES
+                            :: validL2PTable(d, a, d[l1pt[i].v].entry.l2pt)
+                            && validL2PTE(d, a, d[l1pt[i].v].entry.l2pt[j]);
+                    calc {
+                        dataPageRefs(dOut, a, p);
+                        dataPageRefs(d, a, p);
+                        ({});
+                    }
+                }
+                assert validPageDbEntryTyped(dOut, n);
+            } else if d[n].entry.DataPage? {
+                assert dOut[n] == d[n];
+                calc {
+                    dataPageRefs(d, a, n);
+                    { assert forall i:PageNr | dOut[i].PageDbEntryTyped?
+                        && i != p :: dOut[i] == d[i]; }
+                    dataPageRefs(dOut, a, n);
+                }
+                assert validPageDbEntryTyped(dOut, n);
+            }
+        }
     }
 }
 
@@ -90,6 +119,44 @@ function svcMapData(d:PageDb, asPg:PageNr, page:word, mapping:word) : (PageDb, w
         var abs_mapping := wordToMapping(mapping);
         var l2pte := SecureMapping(page, abs_mapping.perm.w, abs_mapping.perm.x);
         var d2 := updateL2Pte(d1, asPg, abs_mapping, l2pte);
+        (d2, KOM_ERR_SUCCESS)
+}
+
+predicate isExistingVAForDataPage(d: PageDb, a: PageNr, mapVA: word, page: PageNr)
+    requires validPageDb(d)
+    requires isAddrspace(d, a) && d[a].entry.state.FinalState?
+    ensures isExistingVAForDataPage(d, a, mapVA, page) ==> validMapping(wordToMapping(mapVA), d, a)
+{
+    reveal validPageDb();
+    reveal wordToMapping();
+
+    var addrspace := d[a].entry;
+    var l1 := d[addrspace.l1ptnr].entry;
+    var l1index := l1indexFromMapping(mapVA);
+    var l2index := l2indexFromMapping(mapVA);
+
+    0 <= l1index < NR_L1PTES
+    && 0 <= l2index < NR_L2PTES
+    && var l1pte := l1.l1pt[l1index]; l1pte.Just?
+    && var l2pt := d[l1pte.v].entry.l2pt; l2pt[l2index].SecureMapping?
+    && l2pt[l2index].page == page
+}
+
+function svcUnmapData(d:PageDb, asPg:PageNr, page:word, mapVA:word) : (PageDb, word)
+    requires validPageDb(d) && validAddrspacePage(d, asPg)
+    requires d[asPg].entry.state.FinalState?
+{
+    reveal validPageDb();
+
+    if !(validPageNr(page) && d[page].PageDbEntryTyped? && d[page].addrspace == asPg
+        && d[page].entry.DataPage?)
+        then (d, KOM_ERR_INVALID_PAGENO)
+    else if !isExistingVAForDataPage(d, asPg, mapVA, page)
+        then (d, KOM_ERR_INVALID_MAPPING)
+    else
+        // revert back to a spare page, and remove the PTE
+        var d1 := updateL2Pte(d, asPg, wordToMapping(mapVA), NoMapping);
+        var d2 := allocateSparePage(d1, page, SparePage);
         (d2, KOM_ERR_SUCCESS)
 }
 
@@ -145,6 +212,9 @@ function svcHandled(s:state, d:PageDb, dispPg:PageNr): (SvcReturnRegs, PageDb)
         (success_regs.(1 := ok), d)
     else if callno == KOM_SVC_MAP_DATA then
         var (retDb, retErr) := svcMapData(d, addrspace, s.regs[R1], s.regs[R2]);
+        (success_regs.(0 := retErr), retDb)
+    else if callno == KOM_SVC_UNMAP_DATA then
+        var (retDb, retErr) := svcUnmapData(d, addrspace, s.regs[R1], s.regs[R2]);
         (success_regs.(0 := retErr), retDb)
     else if callno == KOM_SVC_INIT_L2PTABLE then
         var (retDb, retErr) := svcInitL2PTable(d, addrspace, s.regs[R1], s.regs[R2]);
