verified/svcapi.i.dfy
@@ -2,18 +2,191 @@ include "svcapi.s.dfy"
 include "pagedb.i.dfy"
 include "mapping.i.dfy"
 
+lemma lemma_nonDataPageRefs(d:PageDb, p:PageNr)
+    requires validPageDb(d) && d[p].PageDbEntryTyped? && !hasStoppedAddrspace(d, p)
+    requires !d[p].entry.DataPage?
+    ensures isAddrspace(d, d[p].addrspace) && dataPageRefs(d, d[p].addrspace, p) == {}
+{
+    reveal validPageDb();
+    var a := d[p].addrspace;
+    var l1ptnr := d[a].entry.l1ptnr;
+    var l1pt := d[l1ptnr].entry.l1pt;
+    assert forall i, j | 0 <= i < NR_L1PTES && l1pt[i].Just? && 0 <= j < NR_L2PTES
+        :: validL2PTable(d, a, d[l1pt[i].v].entry.l2pt)
+        && validL2PTE(d, a, d[l1pt[i].v].entry.l2pt[j]);
+}
+
 lemma lemma_svcMapData_validPageDb(d:PageDb, asPg:PageNr, page:word, mapping:word)
     requires validPageDb(d) && validAddrspacePage(d, asPg)
     ensures validPageDb(svcMapData(d, asPg, page, mapping).0)
 {
+    reveal validPageDb();
     var rd := svcMapData(d, asPg, page, mapping).0;
     if rd != d {
         var datapg := DataPage(SeqRepeat(PAGESIZE/WORDSIZE, 0));
         var abs_mapping := wordToMapping(mapping);
+        assert validAndEmptyMapping(abs_mapping, d, asPg)
+            by { reveal wordToMapping(); }
         var l2pte := SecureMapping(page, abs_mapping.perm.w, abs_mapping.perm.x);
         lemma_allocateSparePage(d, page, datapg);
+        lemma_nonDataPageRefs(d, page);
         lemma_updateL2PtePreservesPageDb(allocateSparePage(d, page, datapg),
             asPg, abs_mapping, l2pte);
+    }
+}
+
+lemma lemma_singletonSet_obvious<T>(s:set<T>, e1:T, e2:T)
+    requires |s| <= 1 && e1 in s && e2 in s
+    ensures e1 == e2 && s == {e1}
+{}
+
+lemma lemma_svcUnmapData_validPageDb(d:PageDb, asPg:PageNr, page:word, mapVA:word)
+    requires validPageDb(d) && validAddrspacePage(d, asPg) && d[asPg].entry.state.FinalState?
+    ensures validPageDb(svcUnmapData(d, asPg, page, mapVA).0)
+{
+    reveal validPageDb();
+    reveal wordToMapping();
+    
+    var rd := svcUnmapData(d, asPg, page, mapVA).0;
+    if rd != d {
+        var l1ptnr := d[asPg].entry.l1ptnr;
+        var l1pt := d[l1ptnr].entry.l1pt;
+        var mapping := wordToMapping(mapVA);
+        var l2ptnr := l1pt[mapping.l1index].v;
+        var l2pt := d[l2ptnr].entry.l2pt;
+        var d1 := updateL2Pte(d, asPg, mapping, NoMapping);
+        //assert d1 == d[l2ptnr := d1[l2ptnr]];
+        var l2pt' := d1[l2ptnr].entry.l2pt;
+        //assert l2pt' == l2pt[mapping.l2index := NoMapping];
+        lemma_updateL2PtePreservesPageDb(d, asPg, mapping, NoMapping);
+        assert rd == allocateSparePage(d1, page, SparePage);
+        //assert rd == d1[page := rd[page]];
+
+        assert forall i, j | 0 <= i < NR_L1PTES && l1pt[i].Just? && 0 <= j < NR_L2PTES
+            :: validL2PTable(d, asPg, d[l1pt[i].v].entry.l2pt)
+            && validL2PTE(d, asPg, d[l1pt[i].v].entry.l2pt[j])
+            && validL2PTable(d1, asPg, d1[l1pt[i].v].entry.l2pt)
+            && validL2PTE(d1, asPg, d1[l1pt[i].v].entry.l2pt[j]);
+
+        var oldRefs := dataPageRefs(d, asPg, page);
+        assert oldRefs == {(mapping.l1index, mapping.l2index)}
+        by {
+            var x := (mapping.l1index, mapping.l2index);
+            assert |oldRefs| <= 1 && x in oldRefs;
+            lemma_singletonSet_obvious(oldRefs, x, x);
+        }
+
+        forall (i1, i2 | 0 <= i1 < NR_L1PTES && 0 <= i2 < NR_L2PTES
+            && l1pt[i1].Just? && var l2e := d1[l1pt[i1].v].entry.l2pt[i2];
+            l2e.SecureMapping?) ensures d1[l1pt[i1].v].entry.l2pt[i2].page != page
+        {
+            if i1 == mapping.l1index && i2 == mapping.l2index {
+                assert d1[l1pt[i1].v].entry.l2pt[i2].NoMapping?;
+            } else {
+                assert l2pt[mapping.l2index].SecureMapping? && l2pt[mapping.l2index].page == page;
+                assert (i1, i2) !in oldRefs;
+                assert d1[l1pt[i1].v].entry.l2pt[i2].page != page;
+            }
+        }
+
+        assert validL2PTable(d1, asPg, d1[l2ptnr].entry.l2pt);
+
+        forall i | 0 <= i < NR_L2PTES
+            ensures validL2PTE(rd, asPg, l2pt'[i])
+            ensures i == mapping.l2index <==> (l2pt[i].SecureMapping? && l2pt[i].page == page)
+            ensures l2pt[i].SecureMapping? ==> dataPageRefs(d1, asPg, l2pt[i].page) == (
+                if i == mapping.l2index then {} else dataPageRefs(d, asPg, l2pt[i].page))
+        {
+            assert validL2PTE(d1, asPg, l2pt[i]);
+            if i == mapping.l2index {
+                assert l2pt[i].SecureMapping? && l2pt[i].page == page;
+            }
+            if l2pt[i].SecureMapping? {
+                var oldRefsI := dataPageRefs(d, asPg, l2pt[i].page);
+                var newRefsI := dataPageRefs(d1, asPg, l2pt[i].page);
+                assert (mapping.l1index, i) in oldRefsI;
+                assert isExistingVAForDataPage(d, asPg, mapVA, page);
+                if l2pt[i].page == page {
+                    assert (mapping.l1index, mapping.l2index) in oldRefsI;
+                    lemma_singletonSet_obvious(oldRefsI, (mapping.l1index, i),
+                                               (mapping.l1index, mapping.l2index));
+                    assert i == mapping.l2index;
+                    assert l2pt'[i] == NoMapping;
+                    assert (mapping.l1index, i) !in newRefsI;
+                    assert (mapping.l1index, i) in oldRefsI;
+                    assert |oldRefsI| == 1;
+                    calc {
+                        newRefsI;
+                        { assert d1[l1ptnr].PageDbEntryTyped? && d1[l1ptnr].entry.L1PTable?
+                            && d1[l1ptnr].entry.l1pt == l1pt; }
+                        (set i1, i2 | 0 <= i1 < NR_L1PTES && 0 <= i2 < NR_L2PTES
+                            && l1pt[i1].Just? && var l2e := d1[l1pt[i1].v].entry.l2pt[i2];
+                            l2e.SecureMapping? && l2e.page == page :: (i1, i2));
+                        ({});
+                    }
+                    assert newRefsI == {};
+                } else {
+                    assert oldRefsI == newRefsI;
+                }
+            }
+        }
+
+        forall (n:PageNr | rd[n].PageDbEntryTyped?)
+            ensures validPageDbEntryTyped(rd, n)
+        {
+            if n == page {
+                assert validPageDbEntryTyped(rd, n);
+            } else if n == l2ptnr {
+                assert rd[n] == d1[n];
+                assert validL2PTable(d1, asPg, d1[l2ptnr].entry.l2pt);
+                assert rd[l2ptnr].entry.l2pt == l2pt';
+                assert validL2PTable(rd, asPg, l2pt');
+                assert validPageDbEntryTyped(rd, n);
+            } else {
+                assert rd[n] == d[n];
+                var an := d[n].addrspace;
+                if d[n].entry.DataPage? {
+                    if !hasStoppedAddrspace(d, n) {
+                        calc {
+                            dataPageRefs(d, an, n);
+                            dataPageRefs(d1, an, n);
+                            { assert forall n:PageNr | n != page :: rd[n] == d1[n]; }
+                            dataPageRefs(rd, an, n);
+                        }
+                    }
+                } else if d[n].entry.Addrspace? {
+                    assert addrspaceRefs(rd, n) == addrspaceRefs(d, n);
+                    assert validPageDbEntryTyped(rd, n);
+                } else if d[n].entry.L2PTable? {
+                    if !hasStoppedAddrspace(d, n) {
+                        calc {
+                            true;
+                            validL2PTable(d, an, d[n].entry.l2pt);
+                            validL2PTable(d1, an, d[n].entry.l2pt);
+                            {
+                                if an == asPg {
+                                    forall i2 | 0 <= i2 < NR_L2PTES && var pte := d[n].entry.l2pt[i2];
+                                               pte.SecureMapping? && pte.page == page
+                                        ensures n == l2ptnr
+                                    {
+                                        //assert oldRefs == dataPageRefs(d, asPg, page);
+                                        // FIXME: nothing in validPageDb says all L2s are linked to the L1
+                                        var i1 :| 0 <= i1 < NR_L1PTES && l1pt[i1] == Just(n);
+                                        assert (i1, i2) in oldRefs;
+                                        assert oldRefs == {(mapping.l1index, mapping.l2index)};
+                                        assert (i1, i2) == (mapping.l1index, mapping.l2index);
+                                    }
+                                } else {
+                                    assert forall pte | pte in d[n].entry.l2pt
+                                        && pte.SecureMapping? :: pte.page != page;
+                                }
+                            }
+                            validL2PTable(rd, an, d[n].entry.l2pt);
+                        }
+                    }
+                }
+            }
+        }
     }
 }
 
@@ -34,7 +207,7 @@ lemma lemma_svcInitL2PTable_validPageDb(d:PageDb, asPg:PageNr, page:word, l1inde
         {
             assert validSparePageForAS(d, asPg, page);
             assert !stoppedAddrspace(d[asPg]);
-            assert validL1PTable(d, l1ptnr);
+            assert validL1PTable(d, asPg, l1pt);
             assert l1pt[i].Just? ==> validL1PTE(d, fromJust(l1pt[i]));
         }
 
@@ -42,7 +215,7 @@ lemma lemma_svcInitL2PTable_validPageDb(d:PageDb, asPg:PageNr, page:word, l1inde
         var d1 := allocateSparePage(d, page, l2pt);
         lemma_allocateSparePage(d, page, l2pt);
         var d2 := installL1PTEInPageDb(d1, l1ptnr, page, l1index);
-        installL1PTEPreservesPageDbValidity(d1, l1ptnr, page, l1index);
+        lemma_installL1PTEPreservesPageDbValidity(d1, asPg, l1ptnr, page, l1index);
     }
 }
 
@@ -64,20 +237,27 @@ lemma lemma_svcHandled_validPageDb(s:state, sd:PageDb, dispPg:PageNr, regs:SvcRe
     } else if s.regs[R0] == KOM_SVC_ATTEST || s.regs[R0] == KOM_SVC_VERIFY_STEP2 {
         assert rd == sd;
     } else if s.regs[R0] == KOM_SVC_VERIFY_STEP0 || s.regs[R0] == KOM_SVC_VERIFY_STEP1 {
-        forall n | validPageNr(n) ensures validPageDbEntry(rd, n)
+        forall n:PageNr | n != dispPg && rd[n].PageDbEntryTyped?
+            ensures validPageDbEntryTyped(rd, n)
         {
-            var e := rd[n];
-            if (e.PageDbEntryTyped?)
-            {
-                var entry := e.entry;
-                if (entry.Addrspace?)
-                {
-                    assert addrspaceRefs(rd, n) == addrspaceRefs(sd, n); // set equality
+            assert rd[n] == sd[n];
+            assert validPageDbEntryTyped(sd, n);
+            var entry := rd[n].entry;
+            if (entry.Addrspace?) {
+                assert addrspaceRefs(rd, n) == addrspaceRefs(sd, n); // set equality
+            } else if (entry.DataPage?) {
+                calc {
+                    dataPageRefs(sd, sd[n].addrspace, n);
+                    { assert forall i:PageNr | rd[i].PageDbEntryTyped?
+                        && i != dispPg :: rd[i] == sd[i]; }
+                    dataPageRefs(rd, rd[n].addrspace, n);
                 }
             }
         }
     } else if s.regs[R0] == KOM_SVC_MAP_DATA {
         lemma_svcMapData_validPageDb(sd, addrspace, s.regs[R1], s.regs[R2]);
+    } else if s.regs[R0] == KOM_SVC_UNMAP_DATA {
+        lemma_svcUnmapData_validPageDb(sd, addrspace, s.regs[R1], s.regs[R2]);
     } else if s.regs[R0] == KOM_SVC_INIT_L2PTABLE {
         lemma_svcInitL2PTable_validPageDb(sd, addrspace, s.regs[R1], s.regs[R2]);
     }
